Move the Eq typeclass to Prelude.v.

src/Build/Task.v
@@ -1,31 +1,85 @@
 Require Import Coq.Vectors.Fin.
 Require Import Data.Maybe.
 Require Import Data.Functor.
+Require Import Control.Applicative.
 Require Import Control.Monad.
 Require Import Control.Monad.State.
 Require Import Build.Store.
+Require Import Prelude.
+Require Coq.Program.Wf.
 
-(* (* The Task abstraction *) *)
-(* Record Task (C : (Type -> Type) -> Type) (K V : Type) := *)
-(*   mkTask {key : K; run : forall F `{C F}, ((K -> F V) -> F V)}. *)
+Definition natPlus n m := n + m.
 
-(* Record Task1 (V : Type) := *)
-(*   mkTask1 { key1 : nat *)
-(*           ; run1 : forall F `{Monad F}, (nat -> F V) -> nat -> Maybe (F V)}. *)
+(* type Task2 c k v = forall f. c f => k -> Maybe ((k -> f v) -> f v) *)
 
-(* Record Task := *)
-(*   mkTask { key : nat *)
-(*          ; run : forall F `{Monad F}, (forall k : nat, k < key -> F unit) -> *)
-(*                                        nat -> *)
-(*                                        Maybe (F unit)}. *)
+(* Definition Task {C : (Type -> Type) -> Type} := forall F `{C F}, *)
+(*   nat -> Maybe ((nat -> F nat) -> F nat). *)
 
-Definition ST := State (Store unit nat unit).
+Definition Task :=
+  nat -> Maybe ((nat -> State (Store unit nat nat) nat) -> State (Store unit nat nat) nat).  
+Definition depth (task : Task) (k : nat) : nat :=
+  match (task k) with
+  | Nothing => 0
+  | Just _  => k
+  end.
 
-(* Record Task := *)
-(*   mkTask { key : nat *)
-(*            ; run (k : nat) : ((k, (k < key)) ->  unit) -> *)
-(*                              Maybe (ST unit)}. *)
+Definition taskOrder (task1 task2 : Task) :=
+  forall k, depth task1 k < depth task2 k.
 
-Record Task :=
-  mkTask { key : nat
-         ; run  : ({k | k < key} -> ST unit) -> Maybe (ST unit)}.
+Open Scope monad_scope.
+
+Lemma t : forall task, forall k1 k2, k1 < k2 -> depth task k1 < depth task k2.
+Admitted.
+
+(* Definition fib : Task := *)
+(*   fun (n : nat) (fetch : nat -> (State (Store unit nat nat) nat)) (n : nat) => *)
+(*     match n with  *)
+(*     | O    => Nothing *)
+(*     | S n' => *)
+(*       match n' with *)
+(*       | O     => Nothing *)
+(*       | S n'' => Just (natPlus <$> (fetch n'') <*> (fetch n')) *)
+(*       end *)
+(*     end. *)
+
+Fixpoint fib (fetch : nat -> (State (Store unit nat nat) nat)) (n : nat) :
+  Maybe (State (Store unit nat nat) nat)  :=
+  match n with
+  | O    => Nothing
+  | S n' =>
+    match n' with
+    | O     => Nothing
+    | S n'' => Just (natPlus <$> (fetch n'') <*> (fetch n'))
+    end
+  end.
+
+Program Fixpoint busyFetch (task : Task) (k : nat) {measure (depth task k)}:
+  (State (Store unit nat nat) nat) :=
+    (* let t := (run task) (fun k' => busyFetch task k') k in *)
+    match task k  with
+    | Nothing  => gets (getValue k)
+    | Just act => undefined
+    end.
+
+Check busyFetch (Task fib).
+
+Program Fixpoint busyFetch (task : Task) (k : nat) {measure (depth task k)}:
+  (State (Store unit nat nat) nat) :=
+    (* let t := (run task) (fun k' => busyFetch task k') k in *)
+    match task k  with
+    | Nothing  => gets (getValue k)
+    | Just act =>
+      (act (fun x => busyFetch task k)) >>=
+          fun v => modify (putValue k v) >> pure v
+    end.
+
+Fixpoint busyFib (n : nat) : State (Store unit nat nat) nat :=
+  match n with
+  | O    =>  gets (getValue 0)
+  | S n' =>
+    match n' with
+    | O    =>  gets (getValue 1)
+    | S n'' => natPlus <$> busyFib n'' <*> busyFib n' >>=
+               fun v => modify (putValue n v) >> pure v
+    end
+  end.
