src/Prelude.v
@@ -1,0 +1,20 @@
+Class Eq (A : Type) := {
+  eqb  : A -> A -> bool
+}.
+
+Infix "==" := eqb (at level 40).
+(* Infix "/=" := neqb (at level 40). *)
+
+Definition undefined {a : Type} : a. Admitted.
+
+Definition const {A B : Type} (x : A) (y : B) : A := x.
+
+Fixpoint eq_nat_impl n m : bool :=
+  match n, m with
+    | O, O => true
+    | O, S _ => false
+    | S _, O => false
+    | S n1, S m1 => eq_nat_impl n1 m1
+  end.
+
+Instance eq_nat : Eq nat := { eqb := eq_nat_impl}.
