src/Eq.v
@@ -1,6 +1,0 @@
-Class Eq (A : Type) := {
-  eqb  : A -> A -> bool
-}.
-
-Infix "==" := eqb (at level 40).
-(* Infix "/=" := neqb (at level 40). *)
